checkpoint

steel/Zeta.Steel.AggregateEpochHashes.fsti
@@ -23,7 +23,7 @@ open Zeta.Steel.Util
 val epoch_hash_size : U32.t
 
 let log_ref = G.ref (Seq.seq log_entry_base)
-let log_refs_t = erased (Map.t thread_id log_ref)
+let log_refs_t = erased (Map.t tid log_ref)
 
 noeq
 type epoch_hashes_t = {
@@ -33,7 +33,9 @@ type epoch_hashes_t = {
 
 let epoch_hashes_repr = IArray.repr M.epoch_id M.epoch_hash
 let epoch_id_hash (x:M.epoch_id) : U32.t = x
-let epoch_hash_perm (k:M.epoch_id) (v:epoch_hashes_t) (c:M.epoch_hash) =
+let epoch_hash_perm (k:M.epoch_id)
+                    (v:epoch_hashes_t)
+                    (c:M.epoch_hash) =
     HA.ha_val v.hadd c.hadd `star`
     HA.ha_val v.hevict c.hevict
 
@@ -45,17 +47,36 @@ let all_epoch_hashes =
     epoch_id_hash
     epoch_hash_perm
 
+let tid_bitmap = Seq.lseq bool (U32.v n_threads)
+let epoch_tid_bitmaps =
+  IArray.tbl
+    #M.epoch_id
+    #(larray bool n_threads)
+    #tid_bitmap
+    epoch_id_hash
+    (fun i -> A.pts_to)
+
 let is_epoch_verified (eid:M.epoch_id) (lve:option M.epoch_id) =
   match lve with
   | None -> false
   | Some eid' -> U32.v eid' >= U32.v eid
 
-let epoch_hash_contributions_t = Map.t (thread_id & M.epoch_id) M.epoch_hash
+let epoch_hash_contributions_t = Map.t M.epoch_id (Seq.lseq M.epoch_hash (U32.v n_threads))
 
-let all_contributions_are_accurate (_:epoch_hashes_repr)
-                                   (_:epoch_hash_contributions_t)
+let aggregate_epoch_hash (e0 e1:M.epoch_hash)
+  : M.epoch_hash
+  = { hadd = HA.aggregate_hashes e0.hadd e1.hadd;
+      hevict = HA.aggregate_hashes e0.hevict e1.hevict}
+
+let aggregate_thread_epoch_hashes (e:M.epoch_id) (contribs:epoch_hash_contributions_t)
+  : M.epoch_hash
+  = Zeta.SeqAux.reduce M.init_epoch_hash aggregate_epoch_hash (Map.sel contribs e)
+
+let all_contributions_are_accurate (global:epoch_hashes_repr)
+                                   (contribs:epoch_hash_contributions_t)
   : prop
-  = True //TODO
+  = forall (e:M.epoch_id). Map.sel global e == aggregate_thread_epoch_hashes e contribs
+
 
 let max_certified_epoch_is (_:epoch_hashes_repr)
                            (_:M.epoch_id)
@@ -64,7 +85,8 @@ let max_certified_epoch_is (_:epoch_hashes_repr)
 
 
 let per_thread_contribution_is_accurate (max:M.epoch_id)
-                                        (tid:thread_id)
+                                        (bitmaps: IArray.repr M.epoch_id tid_bitmap)
+                                        (tid:tid)
                                         (entries:Seq.seq log_entry_base)
                                         (contribs:epoch_hash_contributions_t)
   : prop
@@ -74,53 +96,91 @@ let per_thread_contribution_is_accurate (max:M.epoch_id)
      | Some e -> U32.v max <= U32.v e //max can't exceed the verified epoch ctr for tid
      ) /\
     (forall (eid:M.epoch_id).
-      let h_contrib = Map.sel contribs (tid, eid) in
+      let h_contrib = Seq.index (Map.sel contribs eid) (U16.v tid) in
       let h_tsm = Map.sel tsm.epoch_hashes eid in
-      if is_epoch_verified eid tsm.last_verified_epoch
-      then h_contrib == h_tsm
-      else h_contrib == M.init_epoch_hash)
+      Seq.index (Map.sel bitmaps eid) (U16.v tid) == is_epoch_verified eid tsm.last_verified_epoch /\
+      (if is_epoch_verified eid tsm.last_verified_epoch
+       then h_contrib == h_tsm
+       else h_contrib == M.init_epoch_hash))
 
+let tid_index = i:U16.t { U16.v i <= U32.v n_threads }
 
-let rec forall_threads_between (tid:thread_id)
-                               (down_to:thread_id { U16.v tid >= U16.v down_to })
-                               (f:thread_id -> vprop)
+noextract
+let n_threads_16 : tid_index = U16.uint_to_t (U32.v n_threads)
+
+let rec forall_threads_between (from:tid_index)
+                               (to:tid_index { U16.v from <= U16.v to })
+                               (f:tid -> vprop)
   : Tot (vprop)
-        (decreases (U16.v tid))
-  = f tid `star`
-    (if tid = down_to then emp
-     else forall_threads_between U16.(tid -^ 1us) down_to f)
+        (decreases (U16.v to - U16.v from))
+  = if from = to then emp
+    else f from `star`
+         forall_threads_between U16.(from +^ 1us) to f
 
-let forall_threads (f:thread_id -> vprop) =
-  forall_threads_between
-    (UInt16.uint_to_t (U32.v n_threads))
-    0us
-    f
+let forall_threads (f:tid -> vprop) =
+  forall_threads_between 0us n_threads_16 f
 
+let per_thread_invariant (log_refs:log_refs_t)
+                         (max:_)
+                         (bitmaps:_)
+                         (contribs:_)
+                         (tid:tid) =
+    let logref = Map.sel log_refs tid in
+    exists_ (fun (entries:_) ->
+      G.pts_to logref half entries `star`
+      pure (per_thread_contribution_is_accurate max bitmaps tid entries contribs))
+
+val take_thread (#o:_) (#p:tid -> vprop) (i:tid)
+  : STGhostT unit o
+    (forall_threads p)
+    (fun _ -> p i `star`
+         forall_threads_between 0us i p `star`
+         forall_threads_between U16.(i +^ 1us) n_threads_16 p)
+
+val put_thread (#o:_) (#p:tid -> vprop) (i:tid)
+  : STGhostT unit o
+    (p i `star`
+     forall_threads_between 0us i p `star`
+     forall_threads_between U16.(i +^ 1us) n_threads_16 p)
+    (fun _ -> forall_threads p)
+
+
+[@@__reduce__]
+let lock_inv_body (log_refs:log_refs_t)
+                  (hashes : all_epoch_hashes)
+                  (tid_bitmaps : epoch_tid_bitmaps)
+                  (max_certified_epoch : R.ref M.epoch_id)
+                  (contributions: G.ref epoch_hash_contributions_t)
+                  (hashes_v:_)
+                  (bitmaps:_)
+                  (max:_)
+                  (contributions_v:_)
+  = IArray.perm hashes hashes_v Set.empty `star`
+    IArray.perm tid_bitmaps bitmaps Set.empty `star`
+    R.pts_to max_certified_epoch full max `star`
+    G.pts_to contributions full contributions_v `star`
+    pure (all_contributions_are_accurate hashes_v contributions_v /\
+          max_certified_epoch_is hashes_v max) `star`
+    forall_threads (per_thread_invariant log_refs max bitmaps contributions_v)
 
 let lock_inv (log_refs:log_refs_t)
              (hashes : all_epoch_hashes)
+             (tid_bitmaps : epoch_tid_bitmaps)
              (max_certified_epoch : R.ref M.epoch_id)
              (contributions: G.ref epoch_hash_contributions_t)
  : vprop
  = exists_ (fun hashes_v ->
+   exists_ (fun bitmaps ->
    exists_ (fun max ->
    exists_ (fun contributions_v ->
-      IArray.perm hashes hashes_v Set.empty `star`
-      R.pts_to max_certified_epoch full max `star`
-      G.pts_to contributions full contributions_v `star`
-      pure (all_contributions_are_accurate hashes_v contributions_v /\
-            max_certified_epoch_is hashes_v max) `star`
-      forall_threads (fun (tid:thread_id) ->
-        let logref = Map.sel log_refs tid in
-        exists_ (fun (entries:_) ->
-            G.pts_to logref half entries `star`
-            pure (per_thread_contribution_is_accurate max tid entries contributions_v))
-      ))))
+     lock_inv_body log_refs hashes tid_bitmaps max_certified_epoch contributions
+                   hashes_v bitmaps max contributions_v))))
 
 noeq
 type aggregate_epoch_hashes (log_refs:log_refs_t) = {
      hashes : all_epoch_hashes;
+     tid_bitmaps : epoch_tid_bitmaps;
      max_certified_epoch : R.ref M.epoch_id;
      contributions: G.ref epoch_hash_contributions_t;
-     lock: Lock.lock (lock_inv log_refs hashes max_certified_epoch contributions)
+     lock: cancellable_lock (lock_inv log_refs hashes tid_bitmaps max_certified_epoch contributions)
 }
