steel/Zeta.Steel.Util.fst
@@ -8,6 +8,8 @@ let full = Steel.FractionalPermission.full_perm
 let half = Steel.FractionalPermission.half_perm full
 let larray t (n:U32.t) = A.larray t (U32.v n)
 
+let sum_halves : squash (sum_perm half half == full) = admit()
+
 assume
 val empty_map (#k:eqtype) (#v:Type) : FStar.Map.t k v
 
@@ -18,3 +20,28 @@ val admit__ (#a:Type)
             (#q:post_t a)
             (_:unit)
   : STF a p q True (fun _ -> False)
+
+assume
+val cancellable_lock (v:vprop) : Type0
+
+assume
+val can_release (#v:vprop) (c:cancellable_lock v) : vprop
+
+assume
+val new_cancellable_lock (v:vprop)
+  : STT (cancellable_lock v) v (fun _ -> emp)
+
+let maybe_acquired (b:bool) (#v:vprop) (c:cancellable_lock v)
+  = if b then (v `star` can_release c) else emp
+
+assume
+val acquire (#v:vprop) (c:cancellable_lock v)
+  : STT bool emp (fun b -> maybe_acquired b c)
+
+assume
+val release (#v:vprop) (c:cancellable_lock v)
+  : STT unit (v `star` can_release c) (fun _ -> emp)
+
+assume
+val cancel (#v:vprop) (c:cancellable_lock v)
+  : STT unit (can_release c) (fun _ -> emp)
